wip on assert by normalization

src/syntax/const.fs
@@ -175,3 +175,11 @@ let range_of_lid   = pconst "range_of"
 let labeled_lid    = pconst "labeled"
 let range_0        = pconst "range_0"
 let guard_free     = pconst "guard_free"
+
+(* Constants for marking terms with normalization hints *)
+let normalize_ty   = pconst "normalize_ty"
+let normalize_tm   = pconst "normalize_tm"
+let step_beta     = pconst "Beta"
+let step_delta    = pconst "Delta"
+let step_iota     = pconst "Iota"
+let step_zeta     = pconst "Zeta"
